Incremental

ShadowInterpMatchCoind.v
@@ -25,7 +25,7 @@ Module StreamTest.
     fix go s :=
       match s with
       | Str snil => Psnil
-  | Str (scons hd tl) => Pscons hd tl (go tl)
+      | Str (scons hd tl) => Pscons hd tl (go tl)
       end.
 
   CoInductive stream {T : Type} := mkStream { obs_st : streamF T stream }.
@@ -232,25 +232,19 @@ Module StreamTest.
     { destruct s'; destruct k; simpl; intuition auto. }
     destruct s'; destruct k; simpl; intuition auto; subst; try congruence;
     try rewrite IHs in *; intuition auto; subst; eauto.
-    match goal with H : _ |- _ => inversion H; subst; eauto end.
+    match goal with H : _ |- _ => revert H end.
+    inversion 1; subst; eauto.
   Qed.
 
-  Lemma eq_stream_le_streamA {T} (s s' : stream T) (EQ : eq_stream s s')
-  : ∀ n, ∃ m,
-      le_streamA (nth_approx s n) (nth_approx s' m).
+  Lemma eq_stream_eq_approx {T} (s s' : stream T) (EQ : eq_stream s s')
+  : ∀ n, nth_approx s n = nth_approx s' n.
   Proof.
-    intros; revert s s' EQ; induction n; simpl; intros.
-    - exists 0; simpl; eauto.
-    - punfold EQ.
-      unfold eq_streamF in EQ.
-      destruct (obs_st s) eqn:OBS.
-      { exists 0; simpl; auto. }
-      { destruct (obs_st s') eqn:OBS'; [contradiction|].
-        destruct EQ as (? & EQ); subst.
-        destruct EQ as [EQ|?]; [|contradiction].
-        destruct (IHn _ _ EQ) as (m & LE).
-        exists (S m).
-        simpl. rewrite OBS'. eauto. }
+    intros; revert s s' EQ; induction n; simpl; intros; auto.
+    punfold EQ. unfold eq_streamF in EQ.
+    destruct (obs_st s) eqn:OBS; destruct (obs_st s') eqn:OBS';
+    auto; destruct EQ; subst.
+    pclearbot.
+    erewrite IHn; eauto.
   Qed.
 
   (* s = s' ↔ ⌊ s ⌋ ≈ ⌊ s' ⌋ *)
@@ -261,7 +255,8 @@ Module StreamTest.
   Proof.
     split; [|intro; apply eq_streamA_eq_stream; intuition auto].
     intro EQ. apply eq_stream_sym in EQ as EQ'.
-    split; apply eq_stream_le_streamA; auto.
+    split; intros; exists n; erewrite eq_stream_eq_approx; eauto.
+    all: apply le_streamA_refl.
   Qed.
 
   Definition stable {T} (s : nat → streamA T) :=
@@ -271,16 +266,12 @@ Module StreamTest.
   Definition stable_le {T} (s : nat → streamA T) (ST : stable s)
   : ∀ n m (LE : n ≤ m), le_streamA (s n) (s m).
   Proof.
-    intro. revert s ST. induction n; simpl.
-    { intros. revert s ST. clear LE.
-      induction m; simpl; [intros; apply le_streamA_refl|].
-      intros. eapply le_streamA_trans; [apply IHm|]; auto.
-      rewrite le_lt_eq. destruct (ST m); eauto. }
-    intros. destruct m; simpl in *; [lia|].
-    apply IHn with (s := fun n => s (S n)); try lia.
-    intro n'. destruct (ST (S n')) as [?|EQ]; eauto.
-    right. intros m' LE'.
-    assert (n' = m' ∨ S n' ≤ m') as [?|?] by lia; eauto.
+    do 2 intro. revert n s ST. induction m; simpl.
+    { intros. assert (n = 0) by lia; subst. apply le_streamA_refl. }
+    intros. inversion LE; subst. apply le_streamA_refl.
+    eapply le_streamA_trans. apply IHm; auto.
+    rewrite le_lt_eq.
+    destruct (ST m); auto.
   Qed.
 
   Lemma nth_approx_stable {T} (s : stream T) :
@@ -428,8 +419,6 @@ End StreamTest.
 
 Definition var := string.
 
-Module simple.
-
 Inductive shdw {vl} :=
   | Rd (x : var)
   | Ap (s : shdw) (v : vl)
@@ -454,21 +443,34 @@ Arguments vl : clear implicits.
 Definition shadow trace := shdw (vl trace).
 Definition env trace := nv (vl trace).
 
+Inductive traceF {trace} :=
+  | Stuck
+  | Ret (v : vl trace)
+  | Step (s : env trace) (k : traceF)
+.
+
+Arguments traceF : clear implicits.
+
 Section ind.
   Context {T : Type}.
   Let Value := vl T.
   Let Env := env T.
   Let Shadow := shadow T.
+  Let TraceF := traceF T.
   Context (Ptr : T → Prop) (tr_ind : ∀ t, Ptr t)
           (Pshdw : Shadow → Prop)
           (Pnv : Env → Prop)
-          (Pvl : Value → Prop).
+          (Pvl : Value → Prop)
+          (PtrF : TraceF → Prop).
   Context (PRd : ∀ x, Pshdw (Rd x))
           (PAp : ∀ s v, Pshdw s → Pvl v → Pshdw (Ap s v)).
   Context (PInit : Pnv Init)
           (Pnv_bd : ∀ x v σ, Pvl v → Pnv σ → Pnv (nv_bd x v σ)).
   Context (Pvl_sh : ∀ s, Pshdw s → Pvl (vl_sh s))
           (Pvl_clos : ∀ x k σ, Ptr k → Pnv σ → Pvl (vl_clos x k σ)).
+  Context (PStuck : PtrF Stuck)
+          (PRet : ∀ v (IHv : Pvl v), PtrF (Ret v))
+          (PStep : ∀ σ t (IHσ : Pnv σ) (IHt : PtrF t), PtrF (Step σ t)).
 
   Definition shdw_ind vl_ind :=
     fix go s : Pshdw s :=
@@ -490,12 +492,19 @@ Section ind.
     | vl_clos x t σ => Pvl_clos x t σ (tr_ind t) (nv_ind vl_ind σ)
     end.
 
+  Fixpoint traceF_ind t : PtrF t :=
+    match t as k return PtrF k with
+    | Stuck => PStuck
+    | Ret v => PRet v (vl_ind v)
+    | Step σ t => PStep σ t (nv_ind vl_ind σ) (traceF_ind t)
+    end.
+
   Lemma pre_val_ind :
-    (∀ s, Pshdw s) ∧ (∀ σ, Pnv σ) ∧ (∀ v, Pvl v).
+    (∀ s, Pshdw s) ∧ (∀ σ, Pnv σ) ∧ (∀ v, Pvl v) ∧ (∀ t, PtrF t).
   Proof.
     pose proof (nv_ind vl_ind).
     pose proof (shdw_ind vl_ind).
-    eauto using vl_ind.
+    eauto using vl_ind, traceF_ind.
   Qed.
 End ind.
 
@@ -520,14 +529,6 @@ Definition ω := Lam "x" (App (Var "x") (Var "x")).
 Definition ι := Lam "x" (Var "x").
 Definition fst' := Lam "x" (Lam "y" (Var "x")).
 
-Inductive traceF {trace} :=
-  | Stuck
-  | Ret (v : vl trace)
-  | Step (s : env trace) (k : traceF)
-.
-
-Arguments traceF : clear implicits.
-
 (* Finite approximation, annotated with source term *)
 Inductive trace := Tr (e : term) (k : nat → traceF trace).
 
@@ -551,34 +552,26 @@ Section trace_ind.
           (PStep : ∀ σ t (IHσ : Pnv σ) (IHt : PtrF t), PtrF (Step σ t)).
   Context (PTr : ∀ e t (IHt : ∀ n, PtrF (t n)), Ptr (Tr e t)).
 
-  Definition traceF_ind (trace_ind : ∀ t, Ptr t) :=
-    let vl_ind' := vl_ind _ trace_ind _ _ _
+  Fixpoint trace_ind (t : trace) :=
+    let traceF_ind' := traceF_ind _ trace_ind _ _ _ _
       PRd PAp
       PInit Pnv_bd
-      Pvl_sh Pvl_clos in
-    let nv_ind' := nv_ind _ _ PInit Pnv_bd vl_ind' in
-    fix go (t : traceF trace) :=
-    match t as k return PtrF k with
-    | Stuck => PStuck
-    | Ret v => PRet v (vl_ind' v)
-    | Step σ t => PStep σ t (nv_ind' σ) (go t)
-    end.
-
-  Fixpoint trace_ind (t : trace) :=
+      Pvl_sh Pvl_clos
+      PStuck PRet PStep in
     match t with
-    | Tr e t => PTr e t (fun n => traceF_ind trace_ind (t n))
+    | Tr e t => PTr e t (fun n => traceF_ind' (t n))
     end.
 
   Lemma val_ind :
     (∀ s, Pshdw s) ∧ (∀ σ, Pnv σ) ∧ (∀ v, Pvl v) ∧ (∀ tF, PtrF tF) ∧ (∀ t, Ptr t).
   Proof.
     pose proof
-      (pre_val_ind _ trace_ind Pshdw Pnv Pvl
+      (pre_val_ind _ trace_ind _ _ _ _
         PRd PAp
         PInit Pnv_bd
-        Pvl_sh Pvl_clos).
-    intuition auto.
-    all: auto using traceF_ind, trace_ind.
+        Pvl_sh Pvl_clos
+        PStuck PRet PStep).
+    intuition (auto using trace_ind).
   Qed.
 End trace_ind.
 
@@ -631,29 +624,58 @@ Section rel.
         end
       end.
 
+  (* partial order between finite approximations *)
+  Definition rel_traceF {tr tr'}
+    (rel_tr : tr → tr' → Prop) :=
+    fix rel_tF (t : traceF tr) (t' : traceF tr') :=
+      match t with
+      | Stuck => True
+      | Ret v =>
+        match t' with
+        | Ret v' => rel_vl rel_tr v v'
+        | _ => False
+        end
+      | Step σ k =>
+        match t' with
+        | Step σ' k' => rel_nv (rel_vl rel_tr) σ σ' ∧ rel_tF k k'
+        | _ => False
+        end
+      end.
+
+  Definition rel_shadow {tr tr'} (r : tr → tr' → Prop) :=
+    rel_shdw (rel_vl r)
+  .
+  Definition rel_env {tr tr'} (r : tr → tr' → Prop) :=
+    rel_nv (rel_vl r)
+  .
+
   Context {tr tr' : Type}
     (r r' : tr → tr' → Prop)
     (LEt : ∀ t t', r t t' → r' t t').
 
-  Definition rel_shdw_monotone (s : shdw (vl tr)) :=
-    ∀ s', rel_shdw (rel_vl r) s s' →
-          rel_shdw (rel_vl r') s s'
+  Definition rel_shadow_monotone (s : shdw (vl tr)) :=
+    ∀ s', rel_shadow r s s' → rel_shadow r' s s'
   .
-  Definition rel_nv_monotone (σ : nv (vl tr)) :=
-    ∀ σ', rel_nv (rel_vl r) σ σ' → rel_nv (rel_vl r') σ σ'
+  Definition rel_env_monotone (σ : nv (vl tr)) :=
+    ∀ σ', rel_env r σ σ' → rel_env r' σ σ'
   .
   Definition rel_vl_monotone (v : vl tr) :=
     ∀ v', rel_vl r v v' → rel_vl r' v v'
   .
+  Definition rel_traceF_monotone (t : traceF tr) :=
+    ∀ t', rel_traceF r t t' → rel_traceF r' t t'
+  .
 
   Lemma rel_monotone :
-    (∀ s, rel_shdw_monotone s) ∧
-    (∀ σ, rel_nv_monotone σ) ∧
-    (∀ v, rel_vl_monotone v).
+    (∀ s, rel_shadow_monotone s) ∧
+    (∀ σ, rel_env_monotone σ) ∧
+    (∀ v, rel_vl_monotone v) ∧
+    (∀ t, rel_traceF_monotone t).
   Proof.
     apply (pre_val_ind _ (fun _ => I));
-    cbv [rel_shdw_monotone rel_nv_monotone rel_vl_monotone];
-    simpl; intros;
+    cbv [rel_shadow_monotone rel_env_monotone rel_vl_monotone rel_traceF_monotone];
+    cbv [rel_shadow rel_env];
+    simpl; intros; auto;
     match goal with
     | _ : match ?x with _ => _ end |- _ =>
       destruct x; intuition auto
@@ -661,35 +683,48 @@ Section rel.
   Qed.
 End rel.
 
-(* partial order between finite approximations *)
-Definition le_traceF {tr}
-  (le_tr : tr → tr → Prop) :=
-  fix le_tF (t t' : traceF tr) :=
-    let le_vl := rel_vl le_tr in
-    match t with
-    | Stuck => True
-    | Ret v =>
-      match t' with
-      | Ret v' => le_vl v v'
-      | _ => False
-      end
-    | Step σ k =>
-      match t' with
-      | Step σ' k' => rel_nv le_vl σ σ' ∧ le_tF k k'
-      | _ => False
-      end
-    end.
+Section wf.
+  Definition wf_shdw {vl} (wf_vl : vl → Prop) :=
+    fix wf (s : shdw vl) : Prop :=
+      match s with
+      | Rd _ => True
+      | Ap f v => wf f ∧ wf_vl v
+      end.
+
+  Definition wf_nv {vl} (wf_vl : vl → Prop) :=
+    fix wf (σ : nv vl) : Prop :=
+      match σ with
+      | Init => True
+      | nv_bd _ v σ => wf_vl v ∧ wf σ
+      end.
+
+  Definition wf_vl {tr} (wf_tr : tr → Prop) :=
+    fix wf (v : vl tr) :=
+      match v with
+      | vl_sh s => wf_shdw wf s
+      | vl_clos x t σ => wf_tr t ∧ wf_nv wf σ
+      end.
+
+  (* partial order between finite approximations *)
+  Definition wf_traceF {tr} (wf_tr : tr → Prop) :=
+    fix wf (t : traceF tr) :=
+      match t with
+      | Stuck => True
+      | Ret v => wf_vl wf_tr v
+      | Step σ k => wf_nv (wf_vl wf_tr) σ ∧ wf k
+      end.
+End wf.
 
 Fixpoint le_trace (t t' : trace) :=
   match t with
   | Tr e k =>
     match t' with
-    | Tr e' k' => e = e' ∧ ∀ n, ∃ m, le_traceF le_trace (k n) (k' m)
+    | Tr e' k' => e = e' ∧ ∀ n, ∃ m, rel_traceF le_trace (k n) (k' m)
     end
   end.
 
 Lemma le_trace_refl :
-  let le_trF := le_traceF le_trace in
+  let le_trF := rel_traceF le_trace in
   let le_vl := rel_vl le_trace in
   let le_nv := rel_nv le_vl in
   let le_shdw := rel_shdw le_vl in
@@ -701,7 +736,7 @@ Lemma le_trace_refl :
 Proof. cbn zeta. apply val_ind; simpl; eauto. Qed.
 
 Lemma le_trace_trans :
-  let le_trF := le_traceF le_trace in
+  let le_trF := rel_traceF le_trace in
   let le_vl := rel_vl le_trace in
   let le_nv := rel_nv le_vl in
   let le_shdw := rel_shdw le_vl in
@@ -727,7 +762,7 @@ Proof.
   | |- rel_vl _ ?v ?v'' =>
     destruct v; simpl in *; intuition eauto;
     subst; destruct v''; intuition eauto
-  | |- le_traceF _ ?tF ?tF'' =>
+  | |- rel_traceF _ ?tF ?tF'' =>
     destruct tF; simpl in *; intuition eauto;
     subst; destruct tF''; intuition eauto
   | |- le_trace ?t ?t'' =>
@@ -745,19 +780,23 @@ Qed.
 
 Section link.
   Context {trace : Type}.
-  Context {T : Type}.
-  Context (link_trace : env trace → trace → (vl trace → T) → T).
+  Context (link_trace : env trace → trace → (vl trace → traceF trace) → traceF trace).
 
   Definition rd x :=
     fix rd (σ : env trace) :=
       match σ with
       | Init => vl_sh (Rd x)
-      | nv_bd x' v σ' =>
-        if x =? x' then v else rd σ'
+      | nv_bd x' v σ' => if x =? x' then v else rd σ'
       end.
 
-  Lemma rd_monotone {r} x σ σ' (REL : rel_nv (rel_vl r) σ σ') :
-    rel_vl r (rd x σ) (rd x σ').
+  Definition ap f a k :=
+    match f with
+    | vl_sh f' => k (vl_sh (Ap f' a))
+    | vl_clos x t σ => link_trace (nv_bd x a σ) t k
+    end.
+
+  Lemma rel_rd {r} x σ σ' (REL : rel_nv (rel_vl r) σ σ')
+  : rel_vl r (rd x σ) (rd x σ').
   Proof.
     revert σ σ' REL.
     refine (fix go σ :=
@@ -778,22 +817,18 @@ Section link.
   Qed.
 
   Definition link_shdw link_value σ0 :=
-    fix link (s : shadow trace) k : T :=
+    fix link (s : shadow trace) k :=
       match s with
       | Rd x => k (rd x σ0)
       | Ap s' v =>
         let k_s f :=
-          let k_v a :=
-            match f with
-            | vl_sh f' => k (vl_sh (Ap f' a))
-            | vl_clos x k' σ => link_trace (nv_bd x a σ) k' k
-            end
+          let k_v a := ap f a k
           in link_value v k_v
         in link s' k_s
       end.
 
   Definition link_nv link_value (σ0 : env trace) :=
-    fix link (σ : env trace) k : T :=
+    fix link (σ : env trace) k : traceF trace :=
       match σ with
       | Init => k σ0
       | nv_bd x v σ' =>
@@ -804,68 +839,231 @@ Section link.
       end.
 
   Definition link_vl σ0 :=
-    fix link (v : vl trace) k : T :=
+    fix link (v : vl trace) k :=
       match v with
       | vl_sh s => link_shdw link σ0 s k
       | vl_clos x t σ =>
         let k_σ σ' := k (vl_clos x t σ')
         in link_nv link σ0 σ k_σ
       end.
+
+  Definition link_tr σ0 :=
+    fix link (t : traceF trace) k :=
+      match t with
+      | Stuck => Stuck
+      | Ret v => link_vl σ0 v k
+      | Step σ t' =>
+        let k_σ σ' := Step σ' (link t' k) in
+        link_nv (link_vl σ0) σ0 σ k_σ
+      end.
 End link.
 
-Definition link_tr link σ0 :=
-  fix go (t : traceF trace) k {struct t} :=
-    let link_value := link_vl link in
-    match t with
-    | Stuck => Stuck
-    | Ret v => link_value σ0 v k
-    | Step σ t' =>
-      let k_σ σ' := Step σ' (go t' k) in
-      link_nv (link_value σ0) σ0 σ k_σ
-    end.
-
-Fixpoint link_trace n :=
+Fixpoint link_traceF n :=
   match n with
   | 0 => fun _ _ _ => Stuck
   | S n' =>
-    link_tr (fun σ0 '(Tr _ t') => link_trace n' σ0 (t' n'))
+    link_tr (fun σ0 '(Tr _ t') => link_traceF n' σ0 (t' n'))
   end.
 
-Definition link_value n :=
-  link_vl (fun σ0 '(Tr _ t') => link_trace n σ0 (t' n))
+Definition link_trace n σ0 '(Tr _ t') :=
+  link_traceF n σ0 (t' n)
 .
 
-Definition link_env n :=
-  fun σ0 => link_nv (link_value n σ0) σ0
+Definition link_value n := link_vl (link_trace n).
+
+Definition link_env {T} link :=
+  fun σ0 => link_nv (trace := T) (link_vl link σ0) σ0
 .
 
-Definition link_shadow n :=
-  fun σ0 => link_shdw
-    (fun σ0 '(Tr _ t') => link_trace n σ0 (t' n))
-    (link_value n σ0)
-    σ0
+Definition link_envA n := link_env (link_trace n).
+
+Definition link_shadow {T} link :=
+  fun σ0 => link_shdw (trace := T) link (link_vl link σ0) σ0
 .
+
+Definition link_shadowA n := link_shadow (link_trace n).
 
 Fixpoint denote (t : term) k {struct t} : nat → traceF trace :=
   match t with
-  | Var x => fun _ =>
+  | Var x =>
     let r := vl_sh (Rd x) in
-    Step Init (k r)
-  | Lam x e => fun n =>
+    fun _ => Step Init (k r)
+  | Lam x e =>
     let E := Tr e (denote e Ret) in
     let r := vl_clos x E Init in
-    Step Init (k r)
+    fun _ => Step Init (k r)
   | App fn arg => fun n =>
     let k_fn f :=
-      let k_arg a :=
-        match f with
-        | vl_sh f' => k (vl_sh (Ap f' a))
-        | vl_clos x (Tr _ t') σ =>
-          link_trace n (nv_bd x a σ) (t' n) k
-        end in
+      let k_arg a := ap (link_trace n) f a k in
       denote arg k_arg n in
     Step Init (denote fn k_fn n)
   end.
+
+Definition wf_trace t :=
+  match t with
+  | Tr e t' => t' = denote e Ret
+  end.
+
+Definition bind k :=
+  fix bind_ (t : traceF trace) :=
+    match t with
+    | Stuck => Stuck
+    | Ret v => k v
+    | Step σ t' => Step σ (bind_ t')
+    end.
+
+Lemma bind_ext k k' (EXT : ∀ v, k v = k' v) :
+  ∀ t, bind k t = bind k' t.
+Proof.
+  refine (fix go t :=
+    match t with
+    | Stuck => eq_refl
+    | Ret v => EXT v
+    | Step σ t' => f_equal (Step σ) (go t')
+    end).
+Qed.
+
+Lemma bind_bind k k' :
+  ∀ t, bind k' (bind k t) = bind (fun v => bind k' (k v)) t.
+Proof.
+  refine (fix go t :=
+    match t with
+    | Stuck => eq_refl
+    | Ret v => eq_refl
+    | Step σ t' => f_equal (Step σ) (go t')
+    end).
+Qed.
+
+Definition link_shadow_ext {T} link s :=
+  ∀ (k : _ → traceF T) k' σ0 (EXT : ∀ v, k v = k' v),
+    link_shadow link σ0 s k = link_shadow link σ0 s k'
+.
+Definition link_env_ext {T} link σ :=
+  ∀ (k : _ → traceF T) k' σ0 (EXT : ∀ v, k v = k' v),
+    link_env link σ0 σ k = link_env link σ0 σ k'
+.
+Definition link_vl_ext {T} link v :=
+  ∀ (k : _ → traceF T) k' σ0 (EXT : ∀ v, k v = k' v),
+    link_vl link σ0 v k = link_vl link σ0 v k'
+.
+Definition link_tr_ext {T} link (t : traceF T) :=
+  ∀ k k' σ0 (EXT : ∀ v, k v = k' v),
+    link_tr link σ0 t k = link_tr link σ0 t k'
+.
+Definition link_trace_ext {T} (link : _ → _ → _ → traceF T) (t : T) :=
+  ∀ (k : vl T → traceF T) k' (σ0 : env T) (EXT : ∀ v, k v = k' v),
+    link σ0 t k = link σ0 t k'
+.
+
+Lemma pre_link_ext {T} link (LINK_EXT : ∀ t, @link_trace_ext T link t) :
+  (∀ s, link_shadow_ext link s) ∧
+  (∀ σ, link_env_ext link σ) ∧
+  (∀ v, link_vl_ext link v) ∧
+  (∀ t, link_tr_ext link t).
+Proof.
+  cbv [link_trace_ext] in *.
+  apply (pre_val_ind _ (fun _ => I));
+  cbv [link_shadow_ext link_env_ext link_vl_ext link_tr_ext];
+  simpl; eauto.
+  - intros. apply H. intros. apply H0. destruct v0; eauto.
+  - intros. apply IHσ. intros. f_equal. auto.
+Qed.
+
+Lemma link_ext n :
+  ∀ t, link_trace_ext (link_trace n) t.
+Proof.
+  induction n; cbv [link_trace_ext];
+  simpl; intros;
+    match goal with t : trace |- _ => destruct t end;
+    auto.
+  apply pre_link_ext; auto.
+Qed.
+
+Definition link_shadow_bind link s :=
+  ∀ k k' σ0,
+    bind k' (link_shadow link σ0 s k) =
+    link_shadow link σ0 s (fun v' => bind k' (k v'))
+.
+Definition link_env_bind link σ :=
+  ∀ k k' σ0,
+    bind k' (link_env link σ0 σ k) =
+    link_env link σ0 σ (fun v' => bind k' (k v'))
+.
+Definition link_vl_bind link v :=
+  ∀ k k' σ0,
+    bind k' (link_vl link σ0 v k) = link_vl link σ0 v (fun v' => bind k' (k v'))
+.
+Definition link_tr_bind link t :=
+  ∀ k k' σ0,
+    bind k' (link_tr link σ0 t k) = link_tr link σ0 t (fun v => bind k' (k v))
+.
+Definition link_trace_bind link (t : trace) :=
+  ∀ k k' (σ0 : env trace),
+    bind k' (link σ0 t k) = link σ0 t (fun v : vl trace => bind k' (k v))
+.
+
+Lemma pre_link_bind link
+  (LINK_EXT : ∀ t, link_trace_ext link t)
+  (LINK_BIND : ∀ t, link_trace_bind link t) :
+  (∀ s, link_shadow_bind link s) ∧
+  (∀ σ, link_env_bind link σ) ∧
+  (∀ v, link_vl_bind link v) ∧
+  (∀ t, link_tr_bind link t).
+Proof.
+  pose proof (pre_link_ext _ LINK_EXT) as (EXTs & EXTσ & EXTv & EXTt).
+  apply (pre_val_ind _ (fun _ => I));
+  cbv [link_shadow_bind link_env_bind link_vl_bind link_tr_bind];
+  simpl; intros; eauto.
+  - rewrite H. apply EXTs. intros.
+    rewrite H0. apply EXTv. destruct v0; auto.
+    intros. apply LINK_BIND.
+  - rewrite H. apply EXTv. intros.
+    rewrite H0. auto.
+  - unfold link_env in *. rewrite IHσ. apply EXTσ. intros.
+    simpl. f_equal. auto.
+Qed.
+
+Lemma link_bind n :
+  ∀ t, link_trace_bind (link_trace n) t.
+Proof.
+  induction n; simpl; destruct t as [e t'];
+  cbv [link_trace_bind]; simpl; auto.
+  apply (pre_link_bind _ (link_ext n) IHn).
+Qed.
+
+Lemma link_bind_Ret n σ t k :
+  link_traceF n σ t k = bind k (link_traceF n σ t Ret).
+Proof.
+  destruct n; simpl; auto.
+  destruct (pre_link_bind _ (link_ext n) (link_bind n)) as (_ & _ & _ & ->).
+  auto.
+Qed.
+
+Lemma denote_ext e :
+  ∀ k k' (EXT : ∀ v, k v = k' v) n, denote e k n = denote e k' n.
+Proof.
+  induction e; simpl; intros; f_equal; auto.
+  apply IHe1; intros.
+  apply IHe2; intros. unfold ap.
+  destruct v; auto. pose proof (link_ext n t k k').
+  destruct t. auto.
+Qed.
+
+Lemma denote_bind e :
+  ∀ k k' n, bind k' (denote e k n) = denote e (fun v => bind k' (k v)) n.
+Proof.
+  induction e; simpl; intros; f_equal; auto.
+  rewrite IHe1. apply denote_ext. intros.
+  rewrite IHe2. apply denote_ext. intros. unfold ap.
+  destruct v; auto. pose proof (link_bind n t k k').
+  destruct t; auto.
+Qed.
+
+Lemma denote_bind_Ret e :
+  ∀ k n, denote e k n = bind k (denote e Ret n).
+Proof.
+  intros. rewrite denote_bind. apply denote_ext. reflexivity.
+Qed.
 
 (* traditional *)
 Inductive value :=
@@ -893,12 +1091,48 @@ Definition ev ev :=
     let k_fn f :=
       let k_arg a :=
         match f with
-        | value_clos x e σ' =>
-          ev e k ((x, a) :: σ')
+        | value_clos x e σ' => ev e k ((x, a) :: σ')
         end in
       go arg k_arg σ in
     go fn k_fn σ
   end.
+
+Lemma ev_ext e :
+  ∀ eval
+    (EVAL_EXT : ∀ t k k' (EXT : ∀ v, k v = k' v) σ,
+      eval t k σ = eval t k' σ)
+    k k' (EXT : ∀ v, k v = k' v) σ,
+    ev eval e k σ = ev eval e k' σ.
+Proof.
+  induction e; simpl; intros; auto.
+  { destruct (rd' _ _); auto. }
+  apply IHe1; auto. intros.
+  apply IHe2; auto. destruct v; auto.
+Qed.
+
+Lemma ev_bind e :
+  ∀ eval
+    (EVAL_EXT : ∀ t k k' (EXT : ∀ v, k v = k' v) σ,
+      eval t k σ = eval t k' σ)
+    (EVAL_BIND : ∀ t k k' σ,
+      match eval t k σ with
+      | Some v' => k' v'
+      | None => None
+      end =
+      eval t (fun v => match k v with Some v' => k' v' | None => None end) σ)
+    k k' σ,
+    match ev eval e k σ with
+    | Some v => k' v
+    | None => None
+    end =
+    ev eval e (fun v => match k v with Some v' => k' v' | None => None end) σ.
+Proof.
+  induction e; simpl; intros; auto.
+  { destruct (rd' _ _); auto. }
+  rewrite IHe1 by auto. apply ev_ext; auto. intros.
+  rewrite IHe2 by auto. apply ev_ext; auto. intros.
+  destruct v; auto.
+Qed.
 
 Fixpoint eval n :=
   match n with
@@ -906,62 +1140,162 @@ Fixpoint eval n :=
   | S n' => ev (eval n')
   end.
 
-Definition lift_shdw lift_vl n :=
-  fix go (s : shadow trace) :=
-    match s with
-    | Rd x => fun σ0 => rd' x σ0
-    | Ap s v => fun σ0 =>
-      match lift_vl v σ0 with
-      | Some a =>
-        match go s σ0 with
-        | Some (value_clos x e σ) =>
-          eval n e Some ((x, a) :: σ)
-        | None => None
-        end
-      | None => None
-      end
-    end.
+Lemma eval_ext n :
+  ∀ e k k' (EXT : ∀ v, k v = k' v) σ,
+    eval n e k σ = eval n e k' σ.
+Proof.
+  induction n; simpl; auto using ev_ext.
+Qed.
 
-Definition lift_nv lift_vl :=
-  fix go (σ : env trace) :=
+Lemma eval_bind n :
+  ∀ e k k' σ,
+    match eval n e k σ with
+    | Some v => k' v
+    | None => None
+    end =
+    eval n e (fun v => match k v with Some v' => k' v' | None => None end) σ.
+Proof.
+  induction n; simpl; auto using eval_ext, ev_bind.
+Qed.
+
+Lemma eval_bind_Some n :
+  ∀ e k σ,
+    eval n e k σ =
+    match eval n e Some σ with
+    | Some v => k v
+    | None => None
+    end.
+Proof.
+  intros. rewrite eval_bind. reflexivity.
+Qed.
+
+Definition lift_nv f :=
+  fix go (σ : list (var * value)) : env trace :=
     match σ with
-    | Init => @Some (list (var * value))
-    | nv_bd x v σ' => fun σ0 =>
-      match lift_vl v σ0 with
-      | Some v' =>
-        match go σ' σ0 with
-        | Some σ'' => Some ((x, v') :: σ'')
-        | None => None
-        end
-      | None => None
-      end
+    | [] => Init
+    | (x, v) :: σ' => nv_bd x (f v) (go σ')
     end.
 
-Definition lift_vl n :=
-  fix go (v : vl trace) :=
-    match v with
-    | vl_sh s => lift_shdw go n s
-    | vl_clos x (Tr e _) σ => fun σ0 =>
-      match lift_nv go σ σ0 with
-      | Some σ' => Some (value_clos x e σ')
-      | None => None
-      end
-    end.
+Fixpoint lift_value v :=
+  match v with
+  | value_clos x e σ =>
+    vl_clos x (Tr e (denote e Ret)) (lift_nv lift_value σ)
+  end.
 
-Definition lift_shadow n := lift_shdw (lift_vl n) n.
-Definition lift_env n := lift_nv (lift_vl n).
+Definition lift_env := lift_nv lift_value.
 
-Definition lift_trace n :=
-  fix go (t : traceF trace) :=
-    match t with
-    | Stuck => fun _ => None
-    | Ret v => lift_vl n v
-    | Step σ t' => fun σ0 =>
-      match lift_env n σ σ0 with
-      | Some _ => go t' σ0
-      | None => None
-      end
-    end.
+Fixpoint ret {T} (t : traceF T) :=
+  match t with
+  | Stuck => None
+  | Ret v => Some v
+  | Step _ t' => ret t'
+  end.
+
+(*(RET : ∀ v, ret (T := trace) (link_env link Σ0 σ0 (fun _ => Ret v)) ≠ None)*)
+Definition link_shadow_link link Σ0 σ0 (s : shadow trace) :=
+  ∀ k K
+    (CONT : ∀ v, link_tr link Σ0 (k v) Ret = link_vl link Σ0 v K),
+    link_tr link Σ0 (link_shadow link σ0 s k) Ret =
+    link_env link Σ0 σ0 (fun σ' => link_shadow link σ' s K)
+.
+Definition link_env_link link Σ0 σ0 (σ : env trace) :=
+  ∀ k K
+    (CONT : ∀ σ'', link_tr link Σ0 (k σ'') Ret = link_env link Σ0 σ'' K),
+    link_tr link Σ0 (link_env link σ0 σ k) Ret =
+    link_env link Σ0 σ0 (fun σ' => link_env link σ' σ K)
+.
+Definition link_vl_link link Σ0 σ0 (v : vl trace) :=
+  ∀ k K
+    (CONT : ∀ v', link_tr link Σ0 (k v') Ret = link_vl link Σ0 v' K),
+    link_tr link Σ0 (link_vl link σ0 v k) Ret =
+    link_env link Σ0 σ0 (fun σ' => link_vl link σ' v K)
+.
+Definition link_tr_link link Σ0 σ0 (t : traceF trace) :=
+  ∀ k K
+    (CONT : ∀ v', link_tr link Σ0 (k v') Ret = link_vl link Σ0 v' K),
+    link_tr link Σ0 (link_tr link σ0 t k) Ret =
+    link_env link Σ0 σ0 (fun σ' => link_tr link σ' t K)
+.
+Definition link_trace_link link Σ0 σ0 (t : trace) :=
+  ∀ k K
+    (CONT : ∀ v', link_tr link Σ0 (k v') Ret = link_vl link Σ0 v' K),
+    link_tr link Σ0 (link σ0 t k) Ret =
+    link_env link Σ0 σ0 (fun σ' => link σ' t K)
+.
+
+Lemma link_rd link
+  (LINK_EXT : ∀ t, link_trace_ext link t)
+  (LINK_BIND : ∀ t, link_trace_bind link t)
+  (Σ0 : env trace) :
+  ∀ σ0 k x
+    (RET : ∀ v, ret (link_env link Σ0 σ0 (fun _ => Ret v)) ≠ None),
+    link_vl link Σ0 (rd x σ0) k = link_env link Σ0 σ0 (fun σ' => k (rd x σ')).
+Proof.
+  pose proof (pre_link_ext _ LINK_EXT) as (_ & _ & EXTv & _).
+  pose proof (pre_link_bind _ LINK_EXT LINK_BIND) as (_ & BINDσ & BINDv & _).
+  cbv [link_env_ext link_vl_bind link_env_bind] in *.
+  refine (fix go σ0 :=
+    match σ0 with
+    | Init => fun k x RET => _
+    | nv_bd x' V Σ' => fun k x RET => _
+    end).
+  { reflexivity. }
+Abort.
+
+Lemma pre_link_link link Σ0 σ0
+  (LINK_EXT : ∀ t, link_trace_ext link t)
+  (LINK_LINK : ∀ t, link_trace_link link Σ0 σ0 t)
+  (RET : ∀ v, ret (link_env link Σ0 σ0 (fun _ => Ret v)) ≠ None) :
+  (∀ s, link_shadow_link link Σ0 σ0 s) ∧
+  (∀ σ, link_env_link link Σ0 σ0 σ) ∧
+  (∀ v, link_vl_link link Σ0 σ0 v) ∧
+  (∀ t, link_tr_link link Σ0 σ0 t).
+Proof.
+  pose proof (pre_link_ext _ LINK_EXT) as (EXTs & EXTσ & EXTv & EXTt).
+  apply (pre_val_ind _ (fun _ => I));
+  cbv [link_shadow_link link_env_link link_vl_link link_tr_link];
+  simpl; intros; eauto.
+  - rewrite CONT. 
+  - rewrite H. apply EXTs. intros.
+    rewrite H0. apply EXTv. destruct v0; auto.
+    intros. apply LINK_BIND.
+  - rewrite H. apply EXTv. intros.
+    rewrite H0. auto.
+  - unfold link_env in *. rewrite IHσ. apply EXTσ. intros.
+    simpl. f_equal. auto.
+Qed.
+
+Lemma lift_link e :
+  ∀ σ0 Σ n,
+  lift_trace (eval n) σ0 (link_traceF (S n) Σ (denote e Ret n) Ret) =
+  match lift_env (eval n) σ0 Σ with
+  | Some Σ0 => ev (eval n) e Some Σ0
+  | None => None
+  end.
+Proof.
+  induction e; simpl; intros.
+  { destruct (lift_env _ _ _) eqn:LIFTΣ; auto. erewrite lift_rd; eauto.
+    destruct (rd' _ _); auto. }
+  { unfold lift_env. destruct (lift_nv _ _ _); auto. }
+  intros.
+  rewrite denote_bind_Ret.
+  erewrite bind_ext; [|intros; rewrite denote_bind_Ret; reflexivity].
+Qed.
+
+
+Definition link_vl_bind link v :=
+  ∀ k k' σ0,
+    bind k' (link_vl link σ0 v k) = link_vl link σ0 v (fun v' => bind k' (k v'))
+.
+Definition link_tr_bind link t :=
+  ∀ k k' σ0,
+    bind k' (link_tr link σ0 t k) = link_tr link σ0 t (fun v => bind k' (k v))
+.
+Definition link_trace_bind link (t : trace) :=
+  ∀ k k' (σ0 : env trace),
+    bind k' (link σ0 t k) = link σ0 t (fun v : vl trace => bind k' (k v))
+.
+
 
 Lemma ev_monotonicity : ∀ e k k' σ v f f'
   (K_MONO : ∀ v w, k v = Some w → k' v = Some w)
@@ -992,811 +1326,94 @@ Proof.
   intros. eapply IHm; eauto. lia.
 Qed.
 
-Definition bind_link_shdw n s :=
-  ∀ σ0 Σ0 σ1 Σ1 k k'
-    (WF : ∀ v0' v1'
-      (LIFT : lift_vl v0' Σ0 = lift_vl v1' Σ1)
-      (VALID : lift_vl v0' Σ0 ≠ None),
-      lift_trace (k v0') Σ0 = lift_trace (k' v1') Σ1)
-    (LIFTΣ : lift_env σ0 Σ0 = lift_env σ1 Σ1)
-    (VALIDΣ : lift_env σ0 Σ0 ≠ None),
-    lift_trace (link_shadow n σ0 s k) Σ0 =
-    lift_trace (link_shadow n σ1 s k') Σ1
-  .
-
-Definition bind_link_nv n σ :=
-  ∀ σ0 Σ0 σ1 Σ1 k k'
-    (WF : ∀ σ0' σ1'
-      (LIFT : lift_env σ0' Σ0 = lift_env σ1' Σ1)
-      (VALID : lift_env σ0' Σ0 ≠ None),
-      lift_trace (k σ0') Σ0 = lift_trace (k' σ1') Σ1)
-    (LIFTΣ : lift_env σ0 Σ0 = lift_env σ1 Σ1)
-    (VALIDΣ : lift_env σ0 Σ0 ≠ None),
-    lift_trace (link_env n σ0 σ k) Σ0 =
-    lift_trace (link_env n σ1 σ k') Σ1
-  .
-
-Definition bind_link_vl n v :=
-  ∀ σ0 Σ0 σ1 Σ1 k k'
-    (WF : ∀ v0' v1'
-      (LIFT : lift_vl v0' Σ0 = lift_vl v1' Σ1)
-      (VALID : lift_vl v0' Σ0 ≠ None),
-      lift_trace (k v0') Σ0 = lift_trace (k' v1') Σ1)
-    (LIFTΣ : lift_env σ0 Σ0 = lift_env σ1 Σ1)
-    (VALIDΣ : lift_env σ0 Σ0 ≠ None),
-    lift_trace (link_value n σ0 v k) Σ0 =
-    lift_trace (link_value n σ1 v k') Σ1
-  .
-
-Definition bind_link_tr n t :=
-  ∀ σ0 Σ0 σ1 Σ1 k k'
-    (WF : ∀ v0' v1'
-      (LIFT : lift_vl v0' Σ0 = lift_vl v1' Σ1)
-      (VALID : lift_vl v0' Σ0 ≠ None),
-      lift_trace (k v0') Σ0 = lift_trace (k' v1') Σ1)
-    (LIFTΣ : lift_env σ0 Σ0 = lift_env σ1 Σ1)
-    (VALIDΣ : lift_env σ0 Σ0 ≠ None),
-    lift_trace (link_trace n σ0 t k) Σ0 =
-    lift_trace (link_trace n σ1 t k') Σ1
-  .
-
-Lemma bind_link m : ∀ n (LE : n ≤ m),
-  (∀ s, bind_link_shdw n s) ∧
-  (∀ σ, bind_link_nv n σ) ∧
-  (∀ v, bind_link_vl n v) ∧
-  (∀ t, bind_link_tr n t) ∧
-  (∀ t, match t with Tr _ t' => bind_link_tr n t' end).
+Lemma base_case e :
+  ∀ Σ0 k K
+    (LIFTK : ∀ V, lift_trace (link_trace 1 Σ0 (K V) Ret) =
+      match lift_trace (link_value 1 Σ0 V Ret) with
+      | Some v => k v
+      | None => None
+      end),
+    lift_trace (link_trace 1 Σ0 (denote e K 0) Ret) =
+    match lift_env Σ0 with
+    | Some σ0 => ev (eval 0) e k σ0
+    | None => None
+    end.
 Proof.
-  induction m.
-  { intros. assert (n = 0) by lia. subst.
-    cbv [bind_link_shdw bind_link_nv bind_link_vl bind_link_tr].
-    simpl. intuition auto. destruct t; auto. }
-  intro. destruct n.
-  { cbv [bind_link_shdw bind_link_nv bind_link_vl bind_link_tr].
-    simpl. intuition auto. destruct t; auto. }
-  intro. apply PeanoNat.Nat.succ_le_mono in LE.
-  specialize (IHm _ LE).
-  destruct IHm as (IHms & IHmσ & IHmv & IHmtF & IHmt).
-  apply val_ind; intros;
-  cbv [bind_link_shdw bind_link_nv bind_link_vl bind_link_tr] in *;
-  simpl; intros; auto.
-  - apply WF. all: admit.
-  - apply IHs; auto. intros.
-    apply IHmv; auto. intros.
-    destruct v0'. { simpl in VALID. congruence. }
-    destruct v1'. { rewrite LIFT in VALID. simpl in *; congruence. }
-    destruct t, t0.
-    apply IHmtF.
-    { destruct v1'; simpl in LIFT. apply WF; auto.
-      destruct t. simpl in 
-      change (lift_nv lift_vl σ Σ1) with (lift_env σ Σ1) in LIFT.
-      destruct (lift_env σ Σ1) eqn:LIFTΣ'. congruence.
-      simpl in VALID. congruence.
-      
-      destruct (lift_nv σ Σ1) in LIFT. }
-  apply IHv; auto. intros.
-    apply LIFT.
-  - apply IHv; auto. intros. apply IHσ; auto.
-    intros. apply WF; auto. simpl.
-    rewrite LIFT, LIFT0. auto.
-  - `:with`
+  induction e; simpl in *.
+  { intros. erewrite LIFTK. destruct (lift_env Σ0) eqn: LIFTΣ; auto.
+    simpl. erewrite lift_rd; eauto. }
+  { intros. erewrite LIFTK. simpl. unfold lift_env.
+    destruct (lift_nv _ Σ0); auto. }
+  intros.
+  destruct (lift_env Σ0) as [σ0|] eqn:LIFTΣ; eauto.
+  erewrite IHe1. rewrite LIFTΣ. eauto.
+  intros. simpl. destruct V as [f' |x e t']; simpl.
+  erewrite IHe2.
+  simpl. erewrite IHe2.
+  specialize (IHe1 Σ0). rewrite LIFTΣ in IHe1.
+  rewrite denote_bind_Ret.
+  pose proof (link_bind_Ret 1) as RR. simpl in RR.
+  rewrite RR. clear RR.
+  destruct (pre_link_bind _ (link_ext 0) (link_bind 0)) as (_ & _ & _ & RR).
+  simpl in RR. rewrite RR.
+  simpl in *.
+  rewrite 
+  rewrite IHe1.
+  rewrite 
+  erewrite IHe1; auto. simpl.
+  intros. erewrite IHe2; cycle 1. instantiate (1 := fun v =>
+    match V with
+    | vl_sh f' => _
+    | _ => None
+    end).
+  simpl.
+  { intros. destruct V; simpl in *. rewrite CONT; simpl; auto.
+    destruct (lift_vl _ _ _); auto.
+    destruct t; destruct (lift_vl _ _ _); auto. }
+  simpl. destruct V as [f'|x (e & t')]; simpl; cycle 1.
+  simpl in WF. destruct WF as (? & WF); subst.
+Admitted.
+
+Lemma test e :
+  ∀ n σ0 k K
+    (LIFT : ∀ V (WF : wf_vl wf_trace V),
+      lift_trace (eval n) (K V) σ0 =
+      match lift_vl (eval n) V σ0 with
+      | None => None
+      | Some v => k v
+      end),
+    ev (ev (eval n)) e k σ0 = lift_trace (eval n) (denote e K n) σ0.
+Proof.
+  induction e; simpl.
+  { intros. rewrite LIFT; simpl; auto. }
+  { intros. rewrite LIFT; simpl; auto. }
+  intros. eapply IHe1. intros.
+  destruct (lift_vl _ _ _) eqn:LIFTV.
+  - symmetry. apply IHe2. intros V' WF'.
+    destruct V as [f'|x (e & t')]; simpl.
+    { rewrite LIFT; simpl; auto.
+      simpl in LIFTV. rewrite LIFTV.
+      destruct (lift_vl _ V' σ0) eqn:LIFTV'; auto.
+      destruct v. admit. }
+  induction n; simpl; [apply base_case|].
+  induction e; simpl; auto.
+  { intros. rewrite LIFT; simpl; auto. }
+  { intros. rewrite LIFT; simpl; auto. }
+  intros. eapply IHe1. intros.
+  destruct (lift_vl _ _ _) eqn:LIFTV.
+  - symmetry. apply IHe2. intros.
+    destruct V; simpl.
+    { rewrite LIFT; simpl; auto.
+      replace (lift_shdw _ _ s σ0) with (Some v).
+      match goal with |- _ = match ?x with _ => _ end => destruct x end;
+      auto.
+      destruct v; auto. admit. }
+    destruct t as (? & t'). simpl in LIFTV.
+    destruct (lift_nv (lift_vl (ev (eval n))) σ σ0) as [Σ|] eqn:LIFTΣ;
+    try congruence.
+    simpl in WF. destruct WF as (? & WF); subst.
+    inversion LIFTV; subst; clear LIFTV.
+    admit.
+  - 
 Abort.
 
-Lemma test' : ∀ n t k k' σ v
-  (EVAL : eval n t k' σ = Some v),
-  lift_trace (denote t k n) σ = Some v.
-Proof.
-  induction n. simpl. congruence.
-  induction t; simpl.
-Abort.
-Module judg.
-(* Judgment *)
-Variant judgF {judg} :=
-  | Stuck
-  | Ret (v : value judg)
-  | AppJ (fn arg body : judg)
-.
-
-Arguments judgF : clear implicits.
-
-Inductive judg := mkJudg (j : judgF judg).
-
-Definition on_ret k :=
-  fix go (j : judg) {struct j} :=
-    let '(mkJudg j') := j in
-    match j' with
-    | Stuck => mkJudg Stuck
-    | Ret v => k v
-    | AppJ _ _ body => go body
-    end.
-
-Definition link_j link σ0 :=
-  let stuck := mkJudg Stuck in
-  let ret v := mkJudg (Ret v) in
-  let appj f a b := mkJudg (AppJ f a b) in
-  fix go (j : judg) k {struct j} :=
-    let '(mkJudg j') := j in
-    match j' with
-    | Stuck => stuck
-    | Ret v => link_vl stuck link σ0 v k
-    | AppJ fn arg _ =>
-      let fn' := go fn ret in
-      let arg' := go arg ret in
-      let k_fn f :=
-        let k_arg a :=
-          match f with
-          | vl_sh s => k (vl_sh (Ap s a))
-          | vl_clos x k' σ => link (nv_bd x a σ) k' k
-          end
-        in on_ret k_arg arg'
-      in appj fn' arg' (on_ret k_fn fn')
-    end.
-
-Definition link_judg :=
-  let stuck := mkJudg Stuck in
-  fix go n :=
-    match n with
-    | 0 => fun _ _ _ => stuck
-    | S n' => link_j (go n')
-    end.
-
-Definition denote_judg :=
-  let stuck := mkJudg Stuck in
-  let ret v := mkJudg (Ret v) in
-  let appj f a b := mkJudg (AppJ f a b) in
-  fix go (t : term) k : nat → judg :=
-    match t with
-    | Var x => fun _ =>
-      let r := vl_sh (Rd x)
-      in k r
-    | Lam x e => fun n =>
-      let r := vl_clos x (go e ret n) Init
-      in k r
-    | App fn arg => fun n =>
-      let fn' := go fn ret n in
-      let arg' := go arg ret n in
-      let k_fn f :=
-        let k_arg a :=
-          match f with
-          | vl_sh f' => k (vl_sh (Ap f' a))
-          | vl_clos x k' σ => link_judg n (nv_bd x a σ) k' k
-          end
-        in on_ret k_arg arg'
-      in appj fn' arg' (on_ret k_fn fn')
-    end.
-
-(* Compute denote_judg (App (App fst' (App ω ω)) ι) (fun r => mkJudg (Ret r)) 2. *)
-End judg.
-
-(* Prove that there exists a unique coinductive tree for every ω chain *)
-End simple.
-
-Definition loc := positive.
-
-Inductive shdw {nv wvl} :=
-  | Init
-  | Rd (s : shdw) (σ : nv) (x : var)
-  | Ap (s : shdw) (w : wvl)
-.
-
-Arguments shdw : clear implicits.
-
-Inductive nv {wvl} :=
-  | nv_sh (s : shdw nv wvl) (* [s] *)
-  | nv_one (x : var) (w : wvl) (* x ↦ w *)
-  | nv_mrg (σ σ' : nv) (* σ ;; σ' *)
-.
-
-Arguments nv : clear implicits.
-
-Variant vl {P wvl tr} :=
-  | vl_prim (p : P) (* primitive Value *)
-  | vl_nv (σ : nv wvl)
-  | vl_sh (s : shdw (nv wvl) wvl) (* s *)
-  | vl_clos (x : var) (t : tr) (σ : nv wvl) (* ⟨ λx.t, σ ⟩ *)
-.
-
-Arguments vl : clear implicits.
-
-Inductive wvl {P tr} :=
-  | wvl_v (v : vl P wvl tr) (* v *)
-  | wvl_recv (v : vl P wvl tr) (* μℓ.v *)
-  | wvl_floc (ℓ : loc) (* free location *)
-  | wvl_bloc (n : nat) (* bound location *)
-.
-
-Arguments wvl : clear implicits.
-
-Variant traceF {P trace} :=
-  | Stuck
-  | Ret (w : wvl P trace)
-  | Step (σ : nv (wvl P trace)) (t : trace)
-.
-
-Arguments traceF : clear implicits.
-
-(* Finite approximation *)
-Inductive trace' {P} := mkTrace' (k : traceF P trace').
-Definition obs_tr' {P} (t : @trace' P) :=
-  match t with
-  | mkTrace' k => k
-  end.
-
-(* Infinite tree *)
-CoInductive trace {P} := mkTrace { obs_tr : traceF P trace }.
-
-Arguments trace' : clear implicits.
-Arguments trace : clear implicits.
-Arguments mkTrace {_} _.
-
-Definition walue := wvl.
-Definition env P trace := nv (walue P trace).
-Definition shadow P trace := shdw (env P trace) (walue P trace).
-Definition value P trace := vl P (walue P trace) trace.
-
-Definition Walue' P := walue P (trace' P).
-Definition Walue P := walue P (trace P).
-Definition Env' P := env P (trace' P).
-Definition Env P := env P (trace P).
-Definition Shadow' P := shadow P (trace' P).
-Definition Shadow P := shadow P (trace P).
-Definition Value' P := value P (trace' P).
-Definition Value P := value P (trace P).
-
-Notation stuck' := (mkTrace' Stuck) (only parsing).
-Notation stuck := (mkTrace Stuck) (only parsing).
-Notation ret' w := (mkTrace' (Ret w)) (only parsing).
-Notation ret w := (mkTrace (Ret w)) (only parsing).
-Notation step' σ t := (mkTrace' (Step σ t)) (only parsing).
-Notation step σ t := (mkTrace (Step σ t)) (only parsing).
-
-Section ind.
-  Context {P tr : Type}.
-  Let Walue := walue P tr.
-  Let Value := value P tr.
-  Let Env := env P tr.
-  Let Shadow := shadow P tr.
-  Context (Ptr : tr → Prop) (tr_ind : ∀ k, Ptr k)
-          (Pshdw : Shadow → Prop)
-          (Pnv : Env → Prop)
-          (Pvl : Value → Prop)
-          (Pwvl : Walue → Prop).
-  Context (PInit : Pshdw Init)
-          (PRd : ∀ s σ x, Pshdw s → Pnv σ → Pshdw (Rd s σ x))
-          (PAp : ∀ s w, Pshdw s → Pwvl w → Pshdw (Ap s w)).
-  Context (Pnv_sh : ∀ s, Pshdw s → Pnv (nv_sh s))
-          (Pnv_one : ∀ x w, Pwvl w → Pnv (nv_one x w))
-          (Pnv_mrg : ∀ σ σ', Pnv σ → Pnv σ' -> Pnv (nv_mrg σ σ')).
-  Context (Pvl_prim : ∀ p, Pvl (vl_prim p))
-          (Pvl_nv : ∀ σ, Pnv σ → Pvl (vl_nv σ))
-          (Pvl_sh : ∀ s, Pshdw s → Pvl (vl_sh s))
-          (Pvl_clos : ∀ x k σ, Ptr k → Pnv σ → Pvl (vl_clos x k σ)).
-  Context (Pwvl_v : ∀ v, Pvl v → Pwvl (wvl_v v))
-          (Pwvl_recv : ∀ v, Pvl v → Pwvl (wvl_recv v))
-          (Pwvl_floc : ∀ ℓ, Pwvl (wvl_floc ℓ))
-          (Pwvl_bloc : ∀ n, Pwvl (wvl_bloc n)).
-
-  Definition shdw_ind nv_ind wvl_ind :=
-    fix go s : Pshdw s :=
-      match s as s' return Pshdw s' with
-      | Init => PInit
-      | Rd s σ x => PRd s σ x (go s) (nv_ind σ)
-      | Ap f w => PAp f w (go f) (wvl_ind w)
-      end.
-
-  Definition nv_ind wvl_ind :=
-    fix go σ : Pnv σ :=
-      match σ as σ' return Pnv σ' with
-      | nv_sh s => Pnv_sh s (shdw_ind go wvl_ind s)
-      | nv_one x w => Pnv_one x w (wvl_ind w)
-      | nv_mrg σ1 σ2 => Pnv_mrg σ1 σ2 (go σ1) (go σ2)
-      end.
-
-  Definition vl_ind wvl_ind v : Pvl v :=
-    match v as v' return Pvl v' with
-    | vl_prim p => Pvl_prim p
-    | vl_nv σ => Pvl_nv σ (nv_ind wvl_ind σ)
-    | vl_sh s => Pvl_sh s (shdw_ind (nv_ind wvl_ind) wvl_ind s)
-    | vl_clos x t σ => Pvl_clos x t σ (tr_ind t) (nv_ind wvl_ind σ)
-    end.
-
-  Fixpoint wvl_ind w : Pwvl w :=
-    match w with
-    | wvl_v v => Pwvl_v v (vl_ind wvl_ind v)
-    | wvl_recv v => Pwvl_recv v (vl_ind wvl_ind v)
-    | wvl_floc ℓ => Pwvl_floc ℓ
-    | wvl_bloc n => Pwvl_bloc n
-    end.
-
-  Lemma pre_val_ind :
-    (∀ s, Pshdw s) ∧ (∀ σ, Pnv σ) ∧ (∀ v, Pvl v) ∧ (∀ w, Pwvl w).
-  Proof.
-    pose proof (nv_ind wvl_ind).
-    pose proof (vl_ind wvl_ind).
-    pose proof (shdw_ind (nv_ind wvl_ind) wvl_ind).
-    eauto using wvl_ind.
-  Qed.
-End ind.
-
-Section trace'_ind.
-  Context {P : Type}.
-  Let tr := trace' P.
-  Let Walue := walue P tr.
-  Let Value := value P tr.
-  Let Env := env P tr.
-  Let Shadow := shadow P tr.
-  Context (Ptr : tr → Prop)
-          (Pshdw : Shadow → Prop)
-          (Pnv : Env → Prop)
-          (Pvl : Value → Prop)
-          (Pwvl : Walue → Prop).
-  Context (PInit : Pshdw Init)
-          (PRd : ∀ s σ x, Pshdw s → Pnv σ → Pshdw (Rd s σ x))
-          (PAp : ∀ s w, Pshdw s → Pwvl w → Pshdw (Ap s w)).
-  Context (Pnv_sh : ∀ s, Pshdw s → Pnv (nv_sh s))
-          (Pnv_one : ∀ x w, Pwvl w → Pnv (nv_one x w))
-          (Pnv_mrg : ∀ σ σ', Pnv σ → Pnv σ' -> Pnv (nv_mrg σ σ')).
-  Context (Pvl_prim : ∀ p, Pvl (vl_prim p))
-          (Pvl_nv : ∀ σ, Pnv σ → Pvl (vl_nv σ))
-          (Pvl_sh : ∀ s, Pshdw s → Pvl (vl_sh s))
-          (Pvl_clos : ∀ x k σ, Ptr k → Pnv σ → Pvl (vl_clos x k σ)).
-  Context (Pwvl_v : ∀ v, Pvl v → Pwvl (wvl_v v))
-          (Pwvl_recv : ∀ v, Pvl v → Pwvl (wvl_recv v))
-          (Pwvl_floc : ∀ ℓ, Pwvl (wvl_floc ℓ))
-          (Pwvl_bloc : ∀ n, Pwvl (wvl_bloc n)).
-  Context (Pstuck : Ptr stuck')
-          (Pret : ∀ w, Pwvl w → Ptr (ret' w))
-          (Pstep : ∀ σ t, Pnv σ → Ptr t → Ptr (step' σ t)).
-
-  Fixpoint trace'_ind (t : tr) : Ptr t :=
-    let wvl_ind' := wvl_ind _ trace'_ind _ _ _ _
-      PInit PRd PAp
-      Pnv_sh Pnv_one Pnv_mrg
-      Pvl_prim Pvl_nv Pvl_sh Pvl_clos
-      Pwvl_v Pwvl_recv Pwvl_floc Pwvl_bloc in
-    let nv_ind' := nv_ind _ _ _
-      PInit PRd PAp
-      Pnv_sh Pnv_one Pnv_mrg wvl_ind' in
-    match t with
-    | mkTrace' k =>
-      match k as k' return Ptr (mkTrace' k') with
-      | Stuck => Pstuck
-      | Ret w => Pret w (wvl_ind' w)
-      | Step σ t => Pstep σ t (nv_ind' σ) (trace'_ind t)
-      end
-    end.
-
-  Lemma val'_ind :
-    (∀ s, Pshdw s) ∧ (∀ σ, Pnv σ) ∧ (∀ v, Pvl v) ∧ (∀ w, Pwvl w) ∧ (∀ t, Ptr t).
-  Proof.
-    pose proof
-      (pre_val_ind (tr := tr) Ptr trace'_ind Pshdw Pnv Pvl Pwvl
-        PInit PRd PAp
-        Pnv_sh Pnv_one Pnv_mrg
-        Pvl_prim Pvl_nv Pvl_sh Pvl_clos
-        Pwvl_v Pwvl_recv Pwvl_floc Pwvl_bloc).
-    intuition auto.
-    apply trace'_ind.
-  Qed.
-End trace'_ind.
-
-Section map.
-  Definition map_shdw {wvl wvl'}
-    (map_wvl : wvl → wvl')
-    (map_nv : nv wvl → nv wvl') :=
-    fix map_s (s : shdw (nv wvl) wvl) : shdw (nv wvl') wvl' :=
-      match s with
-      | Init => Init
-      | Rd s' σ x => Rd (map_s s') (map_nv σ) x
-      | Ap f w => Ap (map_s f) (map_wvl w)
-      end.
-
-  Definition map_nv {wvl wvl'}
-    (map_wvl : wvl → wvl') :=
-    fix map_nv (σ : nv wvl) : nv wvl' :=
-      match σ with
-      | nv_sh s => nv_sh (map_shdw map_wvl map_nv s)
-      | nv_one x w => nv_one x (map_wvl w)
-      | nv_mrg σ1 σ2 => nv_mrg (map_nv σ1) (map_nv σ2)
-      end.
-
-  Definition map_vl {P wvl wvl' tr tr'}
-    (map_wvl : wvl → wvl')
-    (map_tr : tr → tr')
-    (v : vl P wvl tr) : vl P wvl' tr' :=
-    match v with
-    | vl_prim p => vl_prim p
-    | vl_nv σ => vl_nv (map_nv map_wvl σ)
-    | vl_sh s => vl_sh (map_shdw map_wvl (map_nv map_wvl) s)
-    | vl_clos x t σ => vl_clos x (map_tr t) (map_nv map_wvl σ)
-    end.
-
-  Definition map_wvl {P tr tr'}
-    (map_tr : tr → tr') :=
-    fix map_w (w : wvl P tr) : wvl P tr' :=
-      match w with
-      | wvl_v v => wvl_v (map_vl map_w map_tr v)
-      | wvl_recv v => wvl_recv (map_vl map_w map_tr v)
-      | wvl_floc ℓ => wvl_floc ℓ
-      | wvl_bloc ℓ => wvl_bloc ℓ
-      end.
-End map.
-
-Section rel.
-  Definition rel_shdw {wvl wvl'}
-    (rel_wvl : wvl → wvl' → Prop)
-    (rel_nv : nv wvl → nv wvl' → Prop) :=
-    fix rel_s (s : shdw (nv wvl) wvl) (s' : shdw (nv wvl') wvl') : Prop :=
-      match s with
-      | Init => match s' with Init => True | _ => False end
-      | Rd s σ x =>
-        match s' with
-        | Rd s' σ' x' => rel_s s s' ∧ rel_nv σ σ' ∧ x = x'
-        | _ => False
-        end
-      | Ap f w =>
-        match s' with
-        | Ap f' w' => rel_s f f' ∧ rel_wvl w w'
-        | _ => False
-        end
-      end.
-
-  Definition rel_nv {wvl wvl'}
-    (rel_wvl : wvl → wvl' → Prop) :=
-    fix rel_nv (σ : nv wvl) (σ' : nv wvl') : Prop :=
-      match σ with
-      | nv_sh s =>
-        match σ' with
-        | nv_sh s' => rel_shdw rel_wvl rel_nv s s'
-        | _ => False
-        end
-      | nv_one x w =>
-        match σ' with
-        | nv_one x' w' => x = x' ∧ rel_wvl w w'
-        | _ => False
-        end
-      | nv_mrg σ1 σ2 =>
-        match σ' with
-        | nv_mrg σ1' σ2' => rel_nv σ1 σ1' ∧ rel_nv σ2 σ2'
-        | _ => False
-        end
-      end.
-
-  Definition rel_vl {P wvl wvl' tr tr'}
-    (rel_wvl : wvl → wvl' → Prop)
-    (rel_tr : tr → tr' → Prop)
-    (v : vl P wvl tr) (v' : vl P wvl' tr') :=
-    match v with
-    | vl_prim p =>
-      match v' with
-      | vl_prim p' => p = p'
-      | _ => False
-      end
-    | vl_nv σ =>
-      match v' with
-      | vl_nv σ' => rel_nv rel_wvl σ σ'
-      | _ => False
-      end
-    | vl_sh s =>
-      match v' with
-      | vl_sh s' => rel_shdw rel_wvl (rel_nv rel_wvl) s s'
-      | _ => False
-      end
-    | vl_clos x t σ =>
-      match v' with
-      | vl_clos x' t' σ' =>
-        x = x' ∧ rel_tr t t' ∧ rel_nv rel_wvl σ σ'
-      | _ => False
-      end
-    end.
-
-  Definition rel_wvl {P tr tr'}
-    (rel_tr : tr → tr' → Prop) :=
-    fix rel_w (w : wvl P tr) (w' : wvl P tr') :=
-      match w with
-      | wvl_v v =>
-        match w' with
-        | wvl_v v' => rel_vl rel_w rel_tr v v'
-        | _ => False
-        end
-      | wvl_recv v =>
-        match w' with
-        | wvl_recv v' => rel_vl rel_w rel_tr v v'
-        | _ => False
-        end
-      (* Assume a fixed allocation function *)
-      | wvl_floc ℓ => match w' with wvl_floc ℓ' => ℓ = ℓ' | _ => False end
-      | wvl_bloc n => match w' with wvl_bloc n' => n = n' | _ => False end
-      end.
-
-  Context {P tr tr' : Type}
-    (r r' : tr → tr' → Prop)
-    (LEt : ∀ t t', r t t' → r' t t').
-
-  Definition rel_shdw_monotone (s : shdw (nv (wvl P tr)) (wvl P tr)) :=
-    ∀ s', rel_shdw (rel_wvl r) (rel_nv (rel_wvl r)) s s' →
-          rel_shdw (rel_wvl r') (rel_nv (rel_wvl r')) s s'
-  .
-  Definition rel_nv_monotone (σ : nv (wvl P tr)) :=
-    ∀ σ', rel_nv (rel_wvl r) σ σ' → rel_nv (rel_wvl r') σ σ'
-  .
-  Definition rel_vl_monotone (v : vl P (wvl P tr) tr) :=
-    ∀ v', rel_vl (rel_wvl r) r v v' → rel_vl (rel_wvl r') r' v v'
-  .
-  Definition rel_wvl_monotone (w : wvl P tr) :=
-    ∀ w', rel_wvl r w w' → rel_wvl r' w w'
-  .
-
-  Lemma rel_monotone :
-    (∀ s, rel_shdw_monotone s) ∧
-    (∀ σ, rel_nv_monotone σ) ∧
-    (∀ v, rel_vl_monotone v) ∧
-    (∀ w, rel_wvl_monotone w).
-  Proof.
-    apply (pre_val_ind _ (fun _ => I));
-    cbv [rel_shdw_monotone rel_nv_monotone rel_vl_monotone rel_wvl_monotone];
-    simpl; intros;
-    match goal with
-    | _ : match ?x with _ => _ end |- _ =>
-      destruct x; intuition auto
-    end.
-  Qed.
-End rel.
-
-(* partial order between finite approximations *)
-Definition le_trace' {P} :=
-  fix le_t (t t' : trace' P) :=
-    let le_wvl := rel_wvl le_t in
-    match obs_tr' t with
-    | Stuck => True
-    | Ret w =>
-      match obs_tr' t' with
-      | Ret w' => le_wvl w w'
-      | _ => False
-      end
-    | Step σ k =>
-      match obs_tr' t' with
-      | Step σ' k' => rel_nv le_wvl σ σ' ∧ le_t k k'
-      | _ => False
-      end
-    end.
-
-Lemma le_trace'_refl {P} :
-  let le_wvl (w : Walue' P) := rel_wvl le_trace' w in
-  let le_vl (v : Value' P) := rel_vl le_wvl le_trace' v in
-  let le_nv (σ : Env' P) := rel_nv le_wvl σ in
-  let le_shdw (s : Shadow' P) := rel_shdw le_wvl le_nv s in
-  (∀ s, le_shdw s s) ∧
-  (∀ σ, le_nv σ σ) ∧
-  (∀ v, le_vl v v) ∧
-  (∀ w, le_wvl w w) ∧
-  (∀ t : trace' P, le_trace' t t).
-Proof. cbn zeta. apply val'_ind; simpl; auto. Qed.
-
-Lemma le_trace'_trans {P} :
-  let le_wvl (w : Walue' P) := rel_wvl le_trace' w in
-  let le_vl (v : Value' P) := rel_vl le_wvl le_trace' v in
-  let le_nv (σ : Env' P) := rel_nv le_wvl σ in
-  let le_shdw (s : Shadow' P) := rel_shdw le_wvl le_nv s in
-  (∀ s' : Shadow' P,
-    ∀ s s'', le_shdw s s' → le_shdw s' s'' → le_shdw s s'') ∧
-  (∀ σ' : Env' P,
-    ∀ σ σ'', le_nv σ σ' → le_nv σ' σ'' → le_nv σ σ'') ∧
-  (∀ v' : Value' P,
-    ∀ v v'', le_vl v v' → le_vl v' v'' → le_vl v v'') ∧
-  (∀ w' : Walue' P,
-    ∀ w w'', le_wvl w w' → le_wvl w' w'' → le_wvl w w'') ∧
-  (∀ t' : trace' P,
-    ∀ t t'', le_trace' t t' → le_trace' t' t'' → le_trace' t t'').
-Proof.
-  cbn zeta. apply val'_ind; simpl; intros;
-  match goal with
-  | |- rel_shdw _ _ ?s ?s'' =>
-    destruct s; simpl in *; intuition eauto;
-    on_ret; destruct s''; intuition eauto
-  | |- rel_nv _ ?σ ?σ'' =>
-    destruct σ; simpl in *; intuition eauto;
-    on_ret; destruct σ''; intuition eauto
-  | |- rel_vl _ _ ?v ?v'' =>
-    destruct v; simpl in *; intuition eauto;
-    on_ret; destruct v''; intuition eauto
-  | |- rel_wvl _ ?w ?w'' =>
-    destruct w; simpl in *; intuition eauto;
-    on_ret; destruct w''; intuition eauto
-  | |- le_trace' ?t ?t'' =>
-    destruct t; simpl in *; intuition eauto;
-    on_ret; destruct t''; intuition eauto
-  end.
-  - destruct k; simpl in *; intuition eauto.
-  - destruct k; simpl in *; intuition eauto.
-    destruct k0; simpl in *; intuition eauto.
-  - destruct k; simpl in *; intuition eauto.
-    destruct k0; simpl in *; intuition eauto.
-Qed.
-
-(* approx t' t : t' is a finite approximation of t *)
-Definition approx {P} :=
-  fix approx (t' : trace' P) (t : trace P) :=
-    let approx_w := rel_wvl approx in
-    match obs_tr' t' with
-    | Stuck => True
-    | Ret w' =>
-      match obs_tr t with
-      | Ret w => approx_w w' w
-      | _ => False
-      end
-    | Step σ' k' =>
-      match obs_tr t with
-      | Step σ k => rel_nv approx_w σ' σ ∧ approx k' k
-      | _ => False
-      end
-    end.
-
-Variant eq_traceF {P} eq : trace P → trace P → Prop :=
-  | eq_stuck : eq_traceF eq stuck stuck
-  | eq_ret w w'
-    (EQw : rel_wvl eq w w')
-  : eq_traceF eq (ret w) (ret w')
-  | eq_step σ σ' k k'
-    (EQσ : rel_nv (rel_wvl eq) σ σ')
-    (EQk : eq k k')
-  : eq_traceF eq (step σ k) (step σ' k')
-.
-
-Arguments eq_traceF : clear implicits.
-
-Lemma eq_traceF_monotone {P} : monotone2 (eq_traceF P).
-Proof.
-  repeat intro. inversion IN; try constructor; on_ret; auto.
-  all: eapply rel_monotone; eauto.
-Qed.
-
-Hint Resolve eq_traceF_monotone : paco.
-Definition eq_trace P := paco2 (eq_traceF P) bot2.
-
-Fixpoint nth_trace {P} (n : nat) (t : trace P) : trace' P :=
-  match n with
-  | 0 => stuck'
-  | S n' =>
-    match obs_tr t with
-    | Stuck => stuck'
-    | Ret w =>
-      let w' := map_wvl (nth_trace n') w in
-      ret' w'
-    | Step σ k =>
-      let σ' := map_nv (map_wvl (nth_trace n')) σ in
-      step' σ' (nth_trace n' k)
-    end
-  end.
-
-Section subst.
-  Context {P trace : Type}.
-  Let Walue := walue P trace.
-  Let Env := env P trace.
-  Let Value := value P trace.
-  Let Shadow := shadow P trace.
-
-  (** Operations for on_retitution *)
-  (* open the bound location i with ℓ *)
-  Definition open_loc_shdw fw fn (i : nat) (ℓ : loc) :=
-    fix open (s : shadow P trace) : Shadow :=
-    match s with
-    | Init => Init
-    | Rd s σ x => Rd (open s) (fn σ) x
-    | Ap s w => Ap (open s) (fw w)
-    end.
-
-  Definition open_loc_nv fw (i : nat) (ℓ : loc) :=
-    fix open (σ : Env) :=
-    match σ with
-    | nv_sh s => nv_sh (open_loc_shdw fw open i ℓ s)
-    | nv_one x w => nv_one x (fw w)
-    | nv_mrg σ σ' => nv_mrg (open σ) (open σ') 
-    end.
-
-  Definition open_loc_vl fw (i : nat) (ℓ : loc) :=
-    let open (v : Value) :=
-      match v with
-      | vl_prim p => vl_prim p
-      | vl_nv σ => vl_nv (open_loc_nv fw i ℓ σ)
-      | vl_sh s => vl_sh (open_loc_shdw fw (open_loc_nv fw i ℓ) i ℓ s)
-      | vl_clos x k σ => vl_clos x k (open_loc_nv fw i ℓ σ)
-      end in
-    open.
-
-  Fixpoint open_loc_walue (i : nat) (ℓ : loc) (w : Walue) : Walue :=
-    match w with
-    | wvl_v v => wvl_v (open_loc_vl (open_loc_walue i ℓ) i ℓ v)
-    | wvl_recv v => wvl_recv (open_loc_vl (open_loc_walue (S i) ℓ) (S i) ℓ v)
-    | wvl_bloc n => if Nat.eqb i n then wvl_floc ℓ else wvl_bloc n
-    | wvl_floc ℓ => wvl_floc ℓ
-    end.
-
-  Definition open_loc_value i ℓ := open_loc_vl (open_loc_walue i ℓ) i ℓ.
-  Definition open_loc_env i ℓ := open_loc_nv (open_loc_walue i ℓ) i ℓ.
-  Definition open_loc_shadow i ℓ := open_loc_shdw (open_loc_walue i ℓ) (open_loc_env i ℓ).
-
-  (* close the free location ℓ with the binding depth i *)
-  Definition close_loc_shdw fw fn (i : nat) (ℓ : loc) :=
-    fix close (s : shadow P trace) : Shadow :=
-    match s with
-    | Init => Init
-    | Rd s σ x => Rd (close s) (fn σ) x
-    | Ap s w => Ap (close s) (fw w)
-    end.
-
-  Definition close_loc_nv fw (i : nat) (ℓ : loc) :=
-    fix close (σ : Env) :=
-    match σ with
-    | nv_sh s => nv_sh (close_loc_shdw fw close i ℓ s)
-    | nv_one x w => nv_one x (fw w)
-    | nv_mrg σ σ' => nv_mrg (close σ) (close σ') 
-    end.
-
-  Definition close_loc_vl fw (i : nat) (ℓ : loc) :=
-    let close (v : Value) :=
-      match v with
-      | vl_prim p => vl_prim p
-      | vl_nv σ => vl_nv (close_loc_nv fw i ℓ σ)
-      | vl_sh s => vl_sh (close_loc_shdw fw (close_loc_nv fw i ℓ) i ℓ s)
-      | vl_clos x k σ => vl_clos x k (close_loc_nv fw i ℓ σ)
-      end in
-    close.
-
-  Fixpoint close_loc_walue (i : nat) (ℓ : loc) (w : Walue) : Walue :=
-    match w with
-    | wvl_v v => wvl_v (close_loc_vl (close_loc_walue i ℓ) i ℓ v)
-    | wvl_recv v => wvl_recv (close_loc_vl (close_loc_walue (S i) ℓ) (S i) ℓ v)
-    | wvl_bloc n => wvl_bloc n
-    | wvl_floc ℓ' => if Pos.eqb ℓ ℓ' then wvl_bloc i else wvl_floc ℓ'
-    end.
-
-  Definition close_loc_value i ℓ := close_loc_vl (close_loc_walue i ℓ) i ℓ.
-  Definition close_loc_env i ℓ := close_loc_nv (close_loc_walue i ℓ) i ℓ.
-  Definition close_loc_shadow i ℓ := close_loc_shdw (close_loc_walue i ℓ) (close_loc_env i ℓ).
-
-  (* open the bound location i with u *)
-  Definition open_wvl_shdw fw fn (i : nat) (u : Walue) :=
-    fix open (s : shadow P trace) : Shadow :=
-    match s with
-    | Init => Init
-    | Rd s σ x => Rd (open s) (fn σ) x
-    | Ap s w => Ap (open s) (fw w)
-    end.
-
-  Definition open_wvl_nv fw (i : nat) (u : Walue) :=
-    fix open (σ : Env) :=
-    match σ with
-    | nv_sh s => nv_sh (open_wvl_shdw fw open i u s)
-    | nv_one x w => nv_one x (fw w)
-    | nv_mrg σ σ' => nv_mrg (open σ) (open σ') 
-    end.
-
-  Definition open_wvl_vl fw (i : nat) (u : Walue) :=
-    let open (v : Value) :=
-      match v with
-      | vl_prim p => vl_prim p
-      | vl_nv σ => vl_nv (open_wvl_nv fw i u σ)
-      | vl_sh s => vl_sh (open_wvl_shdw fw (open_wvl_nv fw i u) i u s)
-      | vl_clos x k σ => vl_clos x k (open_wvl_nv fw i u σ)
-      end in
-    open.
-
-  Fixpoint open_wvl_walue (i : nat) (u : Walue) (w : Walue) : Walue :=
-    match w with
-    | wvl_v v => wvl_v (open_wvl_vl (open_wvl_walue i u) i u v)
-    | wvl_recv v => wvl_recv (open_wvl_vl (open_wvl_walue (S i) u) (S i) u v)
-    | wvl_bloc n => if Nat.eqb i n then u else wvl_bloc n
-    | wvl_floc ℓ => wvl_floc ℓ
-    end.
-
-  Definition open_wvl_value i ℓ := open_wvl_vl (open_wvl_walue i ℓ) i ℓ.
-  Definition open_wvl_env i ℓ := open_wvl_nv (open_wvl_walue i ℓ) i ℓ.
-  Definition open_wvl_shadow i ℓ := open_wvl_shdw (open_wvl_walue i ℓ) (open_wvl_env i ℓ).
-End subst.
-
-(* Define : coinductive version of traces *)
-(* Define : strong bisimilarity between traces *)
-(* Define : depth-n approximation between traces *)
-(* Prove : strong bisimilarity ↔ equality of approximation for all n *)
-(* Conclusion : represent coinductive trace with a stream of "increasing" approximations *)
